theories/TRAKHTENBROT/membership.v
@@ -12,23 +12,30 @@ Require Import List Arith Nat Lia Max Wellfounded Coq.Setoids.Setoid.
 From Undecidability.Shared.Libs.DLW.Utils 
   Require Import utils_tac utils_list finite.
 
+From Undecidability.Shared.Libs.DLW.Vec 
+  Require Import pos vec.
+
 From Undecidability.TRAKHTENBROT
-  Require Import notations fol_ops.
+  Require Import notations fol_ops fo_terms fo_logic.
 
 Set Implicit Arguments.
 
 Section membership.
 
-  Variable (X : Type) (R : X -> X -> Prop).
+  (** We develop a theory of finitary and computable and 
+      extensional membership. We build pair, ordered pairs
+      and ordered triples and show their properties *)
 
-  Infix "∈" := R.
+  Variable (X : Type) (mem : X -> X -> Prop).
+
+  Infix "∈" := mem.
   Notation "x ∉ y" := (~ x ∈ y).
 
-  Definition m2_incl x y := forall a, a ∈ x -> a ∈ y.
-  Definition m2_equiv x y := forall a, a ∈ x <-> a ∈ y.
+  Definition mb_incl x y := forall a, a ∈ x -> a ∈ y.
+  Definition mb_equiv x y := forall a, a ∈ x <-> a ∈ y.
 
-  Infix "⊆" := m2_incl.
-  Infix "≈" := m2_equiv. 
+  Infix "⊆" := mb_incl.
+  Infix "≈" := mb_equiv. 
   Notation "x ≉ y" := (~ x ≈ y).
 
   (** Hypothesis on the model *)
@@ -38,13 +45,13 @@ Section membership.
   Let lX : list X := proj1_sig Xfin.
   Let HX : forall x, In x lX := proj2_sig Xfin.
 
-  Fact m2_incl_refl x : x ⊆ x.
+  Fact mb_incl_refl x : x ⊆ x.
   Proof. red; auto. Qed.
 
-  Fact m2_incl_trans x y z : x ⊆ y -> y ⊆ z -> x ⊆ z.
-  Proof. unfold m2_incl; auto. Qed.
+  Fact mb_incl_trans x y z : x ⊆ y -> y ⊆ z -> x ⊆ z.
+  Proof. unfold mb_incl; auto. Qed.
 
-  Fact m2_incl_choose x y : { z | z ∈ x /\ z ∉ y } + { x ⊆ y }.
+  Fact mb_incl_choose x y : { z | z ∈ x /\ z ∉ y } + { x ⊆ y }.
   Proof.
     set (P z := z ∈ x /\ z ∉ y).
     set (Q z := z ∈ x -> z ∈ y).
@@ -55,224 +62,138 @@ Section membership.
     + right; intros z; apply H; auto.
   Qed.  
 
-  Fact m2_incl_dec x y : { x ⊆ y } + { ~ x ⊆ y }.
+  Fact mb_incl_dec x y : { x ⊆ y } + { ~ x ⊆ y }.
   Proof.
-    destruct (m2_incl_choose x y) as [ (?&?&?) |]; auto.
+    destruct (mb_incl_choose x y) as [ (?&?&?) |]; auto.
   Qed.
 
-  Fact m2_equiv_eq x y : x ≈ y <-> x ⊆ y /\ y ⊆ x.
+  Fact mb_equiv_eq x y : x ≈ y <-> x ⊆ y /\ y ⊆ x.
   Proof. firstorder. Qed.
   
-  Fact m2_equiv_dec x y : { x ≈ y } + { x ≉ y }.
+  Fact mb_equiv_dec x y : { x ≈ y } + { x ≉ y }.
   Proof.
-    destruct (m2_incl_dec x y); [ destruct (m2_incl_dec y x) | ].
-    1: left; apply m2_equiv_eq; auto. 
-    all: right; rewrite m2_equiv_eq; tauto.
+    destruct (mb_incl_dec x y); [ destruct (mb_incl_dec y x) | ].
+    1: left; apply mb_equiv_eq; auto. 
+    all: right; rewrite mb_equiv_eq; tauto.
   Qed.
 
-  Hint Resolve m2_equiv_dec.
+  Hint Resolve mb_equiv_dec.
 
-  Fact m2_equiv_refl_True x : x ≈ x <-> True.
-  Proof. unfold m2_equiv; tauto. Qed.
+  Fact mb_equiv_refl_True x : x ≈ x <-> True.    Proof. unfold mb_equiv; tauto. Qed.
+  Fact mb_equiv_refl x : x ≈ x.                  Proof. unfold mb_equiv; tauto. Qed.
 
-  Fact m2_equiv_refl x : x ≈ x.
-  Proof. unfold m2_equiv; tauto. Qed.
+  Fact mb_equiv_sym x y : x ≈ y -> y ≈ x.
+  Proof. do 2 rewrite mb_equiv_eq; tauto. Qed.
 
-  Fact m2_equiv_sym x y : x ≈ y -> y ≈ x.
-  Proof. do 2 rewrite m2_equiv_eq; tauto. Qed.
+  Fact mb_equiv_trans x y z : x ≈ y -> y ≈ z -> x ≈ z.
+  Proof. repeat rewrite mb_equiv_eq; unfold mb_incl; intros [] []; split; auto. Qed.
 
-  Fact m2_equiv_trans x y z : x ≈ y -> y ≈ z -> x ≈ z.
-  Proof. repeat rewrite m2_equiv_eq; unfold m2_incl; intros [] []; split; auto. Qed.
+  Add Parametric Relation: (X) (mb_equiv)
+      reflexivity proved by mb_equiv_refl
+      symmetry proved by mb_equiv_sym
+      transitivity proved by mb_equiv_trans
+    as mb_equiv_equivalence.
 
-  Add Parametric Relation: (X) (m2_equiv)
-      reflexivity proved by m2_equiv_refl
-      symmetry proved by m2_equiv_sym
-      transitivity proved by m2_equiv_trans
-    as m2_equiv_rst.
-
-  Hint Resolve m2_equiv_refl m2_equiv_sym.
+  Hint Resolve mb_equiv_refl mb_equiv_sym.
 
   (* A first FOL axiom: sets are characterized by their elements *)
 
-  Definition m2_member_ext := forall x y z, x ≈ y -> x ∈ z -> y ∈ z.
+  Definition mb_member_ext := forall x y z, x ≈ y -> x ∈ z -> y ∈ z.
 
-  Variable (m2_ax_ext : m2_member_ext).
+  Variable (mb_axiom_ext : mb_member_ext).
 
-  Fact m2_equiv_mem x y : x ≈ y -> forall z, x ∈ z <-> y ∈ z.
-  Proof. split; apply m2_ax_ext; auto. Qed.
+  Fact mb_equiv_mem x y : x ≈ y -> forall z, x ∈ z <-> y ∈ z.
+  Proof. split; apply mb_axiom_ext; auto. Qed.
   
-   Add Parametric Morphism: (R) with signature 
-     (m2_equiv) ==> (m2_equiv) ==> (iff) as mem_congr.
+   Add Parametric Morphism: (mem) with signature 
+     (mb_equiv) ==> (mb_equiv) ==> (iff) as mb_mem_congruence.
   Proof.
     intros x y H1 a b H2; red in H1, H2; split;
-     rewrite <- H2; apply m2_ax_ext; auto.
+     rewrite <- H2; apply mb_axiom_ext; auto.
   Qed.
 
   Add Parametric Morphism: (fun x y => x ⊆ y) with signature 
-     (m2_equiv) ==> (m2_equiv) ==> (iff) as is_incl_congr.
+     (mb_equiv) ==> (mb_equiv) ==> (iff) as mb_incl_congruence.
   Proof.
     intros x y H1 a b H2; split; intros H z.
     + rewrite <- H1, <- H2; auto.
     + rewrite H1, H2; auto.
   Qed.
 
-  Definition m2_is_pair p x y := forall a, a ∈ p <-> a ≈ x \/ a ≈ y.
+  Definition mb_is_pair p x y := forall a, a ∈ p <-> a ≈ x \/ a ≈ y.
 
-  Fact m2_is_pair_comm p x y : m2_is_pair p x y -> m2_is_pair p y x.
-  Proof. unfold m2_is_pair; apply forall_equiv; intro; tauto. Qed.
+  Fact mb_is_pair_comm p x y : mb_is_pair p x y -> mb_is_pair p y x.
+  Proof. unfold mb_is_pair; apply forall_equiv; intro; tauto. Qed.
 
-  Add Parametric Morphism: (m2_is_pair) with signature 
-     (m2_equiv) ==> (m2_equiv) ==> (m2_equiv) ==> (iff) as is_pair_congr.
+  Add Parametric Morphism: (mb_is_pair) with signature 
+     (mb_equiv) ==> (mb_equiv) ==> (mb_equiv) ==> (iff) as mb_is_pair_congruence.
   Proof.
     intros p q H1 x x' H2 y y' H3.
     apply forall_equiv; intros a.
     rewrite H1, H2, H3; tauto.
   Qed.
 
-  Fact m2_is_pair_fun p q x y : m2_is_pair p x y -> m2_is_pair q x y -> p ≈ q.
-  Proof.
-    intros H1 H2; red in H1, H2; intro; 
-    rewrite H1, H2; tauto.
-  Qed.
+  Fact mb_is_pair_fun p q x y : mb_is_pair p x y -> mb_is_pair q x y -> p ≈ q.
+  Proof. intros H1 H2; red in H1, H2; intro; rewrite H1, H2; tauto. Qed.
 
-  Fact m2_is_pair_inj p x y x' y' : m2_is_pair p x y 
-                                 -> m2_is_pair p x' y' 
+  (** Many cases here, automation helps !! *)
+
+  Fact mb_is_pair_inj p x y x' y' : mb_is_pair p x y 
+                                 -> mb_is_pair p x' y' 
                                  -> x ≈ x' /\ y ≈ y'
                                  \/ x ≈ y' /\ y ≈ x'.
   Proof.
-    unfold m2_is_pair; intros H1 H2.
-    generalize (proj1 (H2 x)) (proj1 (H2 y)); rewrite H1, H1, m2_equiv_refl_True, m2_equiv_refl_True.
-    generalize (proj1 (H1 x')) (proj1 (H1 y')); rewrite H2, H2, m2_equiv_refl_True, m2_equiv_refl_True.
+    unfold mb_is_pair; intros H1 H2.
+    generalize (proj1 (H2 x)) (proj1 (H2 y)); rewrite H1, H1, mb_equiv_refl_True, mb_equiv_refl_True.
+    generalize (proj1 (H1 x')) (proj1 (H1 y')); rewrite H2, H2, mb_equiv_refl_True, mb_equiv_refl_True.
     intros [] [] [] []; auto.
   Qed.
 
-  Fact m2_is_pair_inj' p x y : m2_is_pair p x x 
-                            -> m2_is_pair p y y
+  Fact mb_is_pair_inj' p x y : mb_is_pair p x x 
+                            -> mb_is_pair p y y
                             -> x ≈ y.
   Proof.
-    intros H1 H2; generalize (m2_is_pair_inj H1 H2); tauto.
+    intros H1 H2; generalize (mb_is_pair_inj H1 H2); tauto.
   Qed.
 
-  Fact m2_is_pair_dec p x y : { m2_is_pair p x y } + { ~ m2_is_pair p x y }.
+  Fact mb_is_pair_dec p x y : { mb_is_pair p x y } + { ~ mb_is_pair p x y }.
   Proof. 
-    unfold m2_is_pair.
+    unfold mb_is_pair.
     apply (fol_quant_sem_dec fol_fa); auto; intros u.
     apply fol_equiv_dec; auto.
     apply (fol_bin_sem_dec fol_disj); auto.
   Qed.
 
-  Hint Resolve m2_is_pair_dec.
+  Hint Resolve mb_is_pair_dec.
 
-  Definition m2_is_triple t x y z := forall a, a ∈ t <-> a ≈ x \/ a ≈ y \/ a ≈ z.
+(*
 
-  Add Parametric Morphism: (m2_is_triple) with signature 
-     (m2_equiv) ==> (m2_equiv) ==> (m2_equiv) ==> (m2_equiv) ==> (iff) as is_triple_congr.
+  Definition mb_is_triple t x y z := forall a, a ∈ t <-> a ≈ x \/ a ≈ y \/ a ≈ z.
+
+  Add Parametric Morphism: (mb_is_triple) with signature 
+     (mb_equiv) ==> (mb_equiv) ==> (mb_equiv) ==> (mb_equiv) ==> (iff) as mb_is_triple_congruence.
   Proof.
     intros p q H1 x x' H2 y y' H3 z z' H4.
     apply forall_equiv; intros a.
     rewrite H1, H2, H3, H4; tauto.
   Qed.
 
-  Fact m2_is_triple_fun r t x y z : m2_is_triple r x y z 
-                                 -> m2_is_triple t x y z 
+  Fact mb_is_triple_fun r t x y z : mb_is_triple r x y z 
+                                 -> mb_is_triple t x y z 
                                  -> r ≈ t.
   Proof.
     intros H1 H2; red in H1, H2; intro;
     rewrite H1, H2; tauto.
   Qed.
 
-  (** Replace the big disj with permutation up-to equivalence *)
-
-  (**
-
-  Ltac collect_equiv :=
-   repeat match goal with 
-     | H : _ ≈ _ |- _ => revert H
-   end.
-
-  Ltac symetry :=
-    repeat match goal with
-      | |- (?x ≈ ?y) -> _ => let H := fresh in intro H; generalize (equiv_sym H); intro
-    end. 
-
-  Ltac eliminate :=
-    repeat match goal with
-      | |- True -> _ => intros _
-      | |- (?x ≈ ?x) -> _ => intros _
-      | |- (?x ≈ ?y) -> _ => let H := fresh in intro H; rewrite H; clear H
-    end. 
-
-  Fact id_rew x : x ≈ x <-> True.
-  Proof. split; auto. Qed.
-
-  Fact True_or_rewl (A : Prop) : A \/ True <-> True.
-  Proof. tauto. Qed.
-
-  Fact True_or_rewr (A : Prop) : True \/ A <-> True.
-  Proof. tauto. Qed.
-
-  Fact True_and_rewl (A : Prop) : A /\ True <-> A.
-  Proof. tauto. Qed.
-
-  Fact True_and_rewr (A : Prop) : True /\ A <-> A.
-  Proof. tauto. Qed.
-
-  Ltac rsimpl := 
-    repeat rewrite id_rew; 
-    repeat (rewrite True_or_rewl  || rewrite True_or_rewr || 
-            rewrite True_and_rewl || rewrite True_and_rewr).
-
-  Ltac myintro :=
-    match goal with
-      | |- True -> _ => intros _ 
-      | |- ?a \/ ?b \/ ?c -> _ => let H := fresh in intros [ H | [ H | H ]]; rewrite H
-    end.
-
-  The idea of encoding a triple as {{x},{x,y},{x,y,z}} seems to generates
-  too many cases to show bijections
-
-  Fact is_triple_inj p x y z x' y' z' : 
-              is_triple p x y z  
-           -> is_triple p x' y' z'
-           -> x ≈ y' /\ y ≈ x' /\ z ≈ z'
-           \/ x ≈ x' /\ y ≈ z' /\ z ≈ y'
-           \/ x ≈ z' /\ y ≈ y' /\ z ≈ x'
-
-           \/ x ≈ x' /\ y ≈ y' /\ z ≈ z'
-           \/ x ≈ y' /\ y ≈ z' /\ z ≈ x'
-           \/ x ≈ z' /\ y ≈ x' /\ z ≈ y'
-
-           \/ x ≈ x' /\ x ≈ y' /\ y ≈ z' /\ z ≈ z'
-           \/ x ≈ x' /\ x ≈ z' /\ y ≈ y' /\ z ≈ y'
-           \/ x ≈ y' /\ x ≈ z' /\ y ≈ x' /\ z ≈ x'
-           \/ x ≈ x' /\ z ≈ x' /\ y ≈ y' /\ y ≈ z'.
-  Proof.
-    unfold is_triple; intros H1 H2.
-    generalize (proj1 (H2 x)) (proj1 (H2 y)) (proj1 (H2 z)); rewrite H1, H1, H1, equiv_refl_True, equiv_refl_True, equiv_refl_True.
-    generalize (proj1 (H1 x')) (proj1 (H1 y')) (proj1 (H1 z')); rewrite H2, H2, H2, equiv_refl_True, equiv_refl_True, equiv_refl_True.
-    clear H1 H2.
-    repeat match goal with 
-     |- (_ -> ?t) -> _ => let H := fresh in let G := fresh in intros H; assert (G : t); [ apply H; auto | ]; clear H
-    end.
-    repeat match goal with H: _ \/ _ \/ _ |- _ => revert H end.
-    repeat (myintro; rsimpl; auto).
-    myintro.
-    
-    do 6 (intros [|[]]; auto; collect_equiv; eliminate; repeat rewrite id_rew; try tauto). [|[]] [|[]] [|[]] [|[]] [|[]]; auto; collect_equiv.
-    eliminate.
-    eliminate.
-    find_trans.
-     match goal with
-      | H : ?x ≈ ?y |- context[?x ≈ ?y] => rewrite (@id_rew x y); auto
-     end.
-  Qed.
 *)
 
+  (** Ordered pairs (x,y) := {{x},{x,y}}, Von Neuman encoding *)
 
-  Definition m2_is_opair p x y := exists a b, m2_is_pair a x x /\ m2_is_pair b x y /\ m2_is_pair p a b.
+  Definition mb_is_opair p x y := exists a b, mb_is_pair a x x /\ mb_is_pair b x y /\ mb_is_pair p a b.
 
-  Add Parametric Morphism: (m2_is_opair) with signature 
-     (m2_equiv) ==> (m2_equiv) ==> (m2_equiv) ==> (iff) as m2_is_opair_congr.
+  Add Parametric Morphism: (mb_is_opair) with signature 
+     (mb_equiv) ==> (mb_equiv) ==> (mb_equiv) ==> (iff) as mb_is_opair_congruence.
   Proof.
     intros p q H1 x x' H2 y y' H3.
     apply exists_equiv; intros a.
@@ -280,99 +201,103 @@ Section membership.
     rewrite H1, H2, H3; tauto.
   Qed.
 
-  Fact m2_is_opair_fun p q x y : m2_is_opair p x y -> m2_is_opair q x y -> p ≈ q.
+  Fact mb_is_opair_fun p q x y : mb_is_opair p x y -> mb_is_opair q x y -> p ≈ q.
   Proof.
     intros (a & b & H1 & H2 & H3) (u & v & G1 & G2 & G3).
-    generalize (m2_is_pair_fun H1 G1) (m2_is_pair_fun H2 G2); intros E1 E2.
+    generalize (mb_is_pair_fun H1 G1) (mb_is_pair_fun H2 G2); intros E1 E2.
     rewrite E1, E2 in H3.
-    revert H3 G3; apply m2_is_pair_fun.
+    revert H3 G3; apply mb_is_pair_fun.
   Qed.
 
-  Fact m2_is_opair_inj p x y x' y' : m2_is_opair p x y 
-                                  -> m2_is_opair p x' y' 
+  Fact mb_is_opair_inj p x y x' y' : mb_is_opair p x y 
+                                  -> mb_is_opair p x' y' 
                                   -> x ≈ x' /\ y ≈ y'.
   Proof.
     intros (a & b & H1 & H2 & H3) (u & v & G1 & G2 & G3).
-    generalize (m2_is_pair_inj H3 G3); intros [ (E1 & E2) | (E1 & E2) ].
+    generalize (mb_is_pair_inj H3 G3); intros [ (E1 & E2) | (E1 & E2) ].
     + rewrite E1 in H1; rewrite E2 in H2.
-      generalize (m2_is_pair_inj' H1 G1); intros E; split; auto.
+      generalize (mb_is_pair_inj' H1 G1); intros E; split; auto.
       rewrite E in H2.
-      generalize (m2_is_pair_inj H2 G2); intros [ | (E3 & E4) ]; try tauto.
+      generalize (mb_is_pair_inj H2 G2); intros [ | (E3 & E4) ]; try tauto.
       rewrite E4; auto.
     + rewrite E1 in H1; rewrite E2 in H2.
-      generalize (m2_is_pair_inj H2 G1) (m2_is_pair_inj H1 G2).
+      generalize (mb_is_pair_inj H2 G1) (mb_is_pair_inj H1 G2).
       intros [ (E3 & E4) | (E3 & E4) ] [ (E5 & E6) | (E5 & E6) ];
         rewrite E4, <- E5; auto.
   Qed.
 
-  Fact m2_is_opair_dec p x y : { m2_is_opair p x y } + { ~ m2_is_opair p x y }.
+  Fact mb_is_opair_dec p x y : { mb_is_opair p x y } + { ~ mb_is_opair p x y }.
   Proof.
-    unfold m2_is_opair.
+    unfold mb_is_opair.
     do 2 (apply (fol_quant_sem_dec fol_ex); auto; intro).
     repeat (apply (fol_bin_sem_dec fol_conj); auto).
   Qed.
 
-  Hint Resolve m2_is_opair_dec.
+  Hint Resolve mb_is_opair_dec.
 
-  Definition m2_is_otriple t x y z := exists p, m2_is_opair p x y /\ m2_is_opair t p z.
+  (** Ordered triples (x,y,z) := ((x,y),z) *)
+
+  Definition mb_is_otriple t x y z := exists p, mb_is_opair p x y /\ mb_is_opair t p z.
  
-  Add Parametric Morphism: (m2_is_otriple) with signature 
-     (m2_equiv) ==> (m2_equiv) ==> (m2_equiv) ==> (m2_equiv) ==> (iff) as m2_is_otriple_congr.
+  Add Parametric Morphism: (mb_is_otriple) with signature 
+     (mb_equiv) ==> (mb_equiv) ==> (mb_equiv) ==> (mb_equiv) ==> (iff) as mb_is_otriple_congruence.
   Proof.
     intros p q H1 x x' H2 y y' H3 z z' H4.
-    unfold m2_is_otriple.
+    unfold mb_is_otriple.
     apply exists_equiv; intros t.
     rewrite H1, H2, H3, H4; tauto.
   Qed.
 
-  Fact m2_is_otriple_fun p q x y z : m2_is_otriple p x y z -> m2_is_otriple q x y z -> p ≈ q.
+  Fact mb_is_otriple_fun p q x y z : mb_is_otriple p x y z -> mb_is_otriple q x y z -> p ≈ q.
   Proof.
     intros (t1 & H1 & H2) (t2 & H3 & H4).
-    generalize (m2_is_opair_fun H1 H3); intros E.
+    generalize (mb_is_opair_fun H1 H3); intros E.
     rewrite E in H2.
-    apply (m2_is_opair_fun H2 H4).
+    apply (mb_is_opair_fun H2 H4).
   Qed.
 
-  Fact m2_is_otriple_inj t x y z x' y' z' : 
-             m2_is_otriple t x y z 
-          -> m2_is_otriple t x' y' z' 
+  Fact mb_is_otriple_inj t x y z x' y' z' : 
+             mb_is_otriple t x y z 
+          -> mb_is_otriple t x' y' z' 
           -> x ≈ x' /\ y ≈ y' /\ z ≈ z'.
   Proof.
     intros (p & H1 & H2) (q & H3 & H4).
-    destruct (m2_is_opair_inj H2 H4) as (H5 & H6).
+    destruct (mb_is_opair_inj H2 H4) as (H5 & H6).
     rewrite H5 in H1.
-    generalize (m2_is_opair_inj H1 H3); tauto.
+    generalize (mb_is_opair_inj H1 H3); tauto.
   Qed.
 
-  Fact m2_is_otriple_dec p x y z : { m2_is_otriple p x y z } + { ~ m2_is_otriple p x y z }.
+  Fact mb_is_otriple_dec p x y z : { mb_is_otriple p x y z } + { ~ mb_is_otriple p x y z }.
   Proof.
     apply (fol_quant_sem_dec fol_ex); auto; intro.
     repeat (apply (fol_bin_sem_dec fol_conj); auto).
   Qed.
 
-  Hint Resolve m2_is_otriple_dec.
+  Hint Resolve mb_is_otriple_dec.
 
-  Definition m2_has_pairs (l : X) :=
-     forall x y, x ∈ l -> y ∈ l -> exists p, m2_is_pair p x y.
+  Definition mb_has_pairs (l : X) :=
+     forall x y, x ∈ l -> y ∈ l -> exists p, mb_is_pair p x y.
 
-  Definition m2_has_otriples (l : X) :=
-    forall x y z, x ∈ l -> y ∈ l -> z ∈ l -> exists t, m2_is_otriple t x y z.
+  Definition mb_has_otriples (l : X) :=
+    forall x y z, x ∈ l -> y ∈ l -> z ∈ l -> exists t, mb_is_otriple t x y z.
 
-  Definition m2_is_otriple_in r x y z :=
-    exists t, m2_is_otriple t x y z /\ t ∈ r.
+  Definition mb_is_otriple_in r x y z :=
+    exists t, mb_is_otriple t x y z /\ t ∈ r.
 
-  Fact m2_is_otriple_in_dec r x y z : { m2_is_otriple_in r x y z } + { ~ m2_is_otriple_in r x y z }.
+  Fact mb_is_otriple_in_dec r x y z : { mb_is_otriple_in r x y z } + { ~ mb_is_otriple_in r x y z }.
   Proof.
     apply (fol_quant_sem_dec fol_ex); auto; intro.
     repeat (apply (fol_bin_sem_dec fol_conj); auto).
   Qed.
 
-  Definition m2_powset (l m : X) := forall x, x ∈ m <-> x ⊆ l.
+(*
 
-  Add Parametric Morphism: (m2_powset) with signature 
-     (m2_equiv) ==> (m2_equiv) ==> (iff) as m2_is_powset_congr.
+  Definition mb_powset (l m : X) := forall x, x ∈ m <-> x ⊆ l.
+
+  Add Parametric Morphism: (mb_powset) with signature 
+     (mb_equiv) ==> (mb_equiv) ==> (iff) as mb_is_powset_congruence.
   Proof.
-    intros x y H1 a b H2; unfold m2_powset.
+    intros x y H1 a b H2; unfold mb_powset.
     apply forall_equiv; intro.
     rewrite H1, H2; tauto.
   Qed.
@@ -382,33 +307,130 @@ Section membership.
   Variable (empty : exists x, forall y, y ∉ x).
  
   Variable (l0 l1 l2 l3 : X).     (** a layered model of level 4 *)
-  Variable (pset1 : m2_powset l0 l1)
-           (pset2 : m2_powset l1 l2)
-           (pset3 : m2_powset l2 l3)
-           (hp0 : m2_has_pairs l0)   (** pairs at every level below 3 *)
-           (hp1 : m2_has_pairs l1)
-           (hp2 : m2_has_pairs l2).
+  Variable (pset1 : mb_powset l0 l1)
+           (pset2 : mb_powset l1 l2)
+           (pset3 : mb_powset l2 l3)
+           (hp0 : mb_has_pairs l0)   (** pairs at every level below 3 *)
+           (hp1 : mb_has_pairs l1)
+           (hp2 : mb_has_pairs l2).
 
-  Fact m2_is_pair_layer p x y l pl : x ∈ l -> y ∈ l -> m2_is_pair p x y -> m2_powset l pl -> p ∈ pl.
+  Fact mb_is_pair_layer p x y l pl : x ∈ l -> y ∈ l -> mb_is_pair p x y -> mb_powset l pl -> p ∈ pl.
   Proof.
     intros H1 H2 H3 H4; apply H4; red in H3.
     intros k; rewrite H3; intros [ H | H ]; rewrite H; auto.
   Qed.
 
-  Fact m2_is_opair_l2 p x y : x ∈ l0 -> y ∈ l0 -> m2_is_opair p x y -> p ∈ l2.
+  Fact mb_is_opair_l2 p x y : x ∈ l0 -> y ∈ l0 -> mb_is_opair p x y -> p ∈ l2.
   Proof.
     intros H1 H2 (a & b & H3 & H4 & H5).
-    apply m2_is_pair_layer with (4 := pset1) in H3; auto.
-    apply m2_is_pair_layer with (4 := pset1) in H4; auto.
-    apply m2_is_pair_layer with (4 := pset2) in H5; auto.
+    apply mb_is_pair_layer with (4 := pset1) in H3; auto.
+    apply mb_is_pair_layer with (4 := pset1) in H4; auto.
+    apply mb_is_pair_layer with (4 := pset2) in H5; auto.
   Qed.
    
   Variable (r : X) (Hr : r ∈ l3). (** r encodes a binary relation *)
 
-  Definition m2_P x y := x ∈ l0 /\ y ∈ l0 /\ exists c, c ∈ r /\ m2_is_opair c x y. 
+  Definition mb_P x y := x ∈ l0 /\ y ∈ l0 /\ exists c, c ∈ r /\ mb_is_opair c x y. 
 
   (** We want to show that (encode A) satisfied in this model
            -> A true in the model where P as defined above 
                 is the binary relation *)
 
-End membership. 
+  *)
+
+End membership.
+
+Section FOL_encoding.
+
+  (** First order encoding here *)
+
+  (** Maybe we can redo the whole devel here with fo_definable.v *)
+
+  Notation Σ2 := (Σrel 2).
+  Variable (Y : Type) (M2 : fo_model Σ2 Y).
+
+  Let mem a b := fom_rels M2 tt (a##b##ø).
+  Notation "x '∈m' y" := (mem x y) (at level 59, no associativity).
+
+  Definition Σ2_mem x y := fol_atom Σ2 tt (£x##£y##ø).
+
+  Infix "∈" := Σ2_mem.
+
+  Definition Σ2_non_empty l := ∃ 0 ∈ (1+l). 
+  Definition Σ2_incl x y := ∀ 0 ∈ (S x) ⤑ 0 ∈ (S y).
+  Definition Σ2_equiv x y := ∀ 0 ∈ (S x) ↔ 0 ∈ (S y).
+
+  Infix "≈" := Σ2_equiv.
+  Infix "⊆" := Σ2_incl.
+
+  Definition Σ2_extensional := ∀∀∀ 2 ≈ 1 ⤑ 2 ∈ 0 ⤑ 1 ∈ 0.
+
+  Definition Σ2_is_pair p x y := ∀ 0 ∈ (S p) ↔ 0 ≈ S x ⟇ 0 ≈ S y.
+
+  Definition Σ2_is_opair p x y := 
+         ∃∃   Σ2_is_pair 1    (2+x) (2+x)
+            ⟑ Σ2_is_pair 0    (2+x) (2+y)
+            ⟑ Σ2_is_pair (2+p) 1     0.
+
+  Definition Σ2_is_otriple p x y z := 
+          ∃   Σ2_is_opair 0     (S x) (S y)
+            ⟑ Σ2_is_opair (S p)  0    (S z).
+
+  Definition Σ2_is_otriple_in r x y z := 
+          ∃   Σ2_is_otriple 0 (S x) (S y) (S z) 
+            ⟑ 0 ∈ (S r).
+
+  Definition Σ2_has_otriples l :=
+        ∀∀∀   2 ∈ (3+l) 
+                      ⤑ 1 ∈ (3+l) 
+                      ⤑ 0 ∈ (3+l) 
+                      ⤑ ∃ Σ2_is_otriple 0 3 2 1.
+
+  (** The formula stating any free variable in list lv has to
+      be interpreted by some element ∈ l *)
+
+  Definition Σ2_list_in l lv := 
+       let f x A := x ∈ l ⟑ A in fold_right f (⊥⤑⊥) lv.
+
+  Variables ψ : nat -> Y.
+
+  Notation "⟪ A ⟫" := (fol_sem M2 ψ A).
+
+  Fact Σ2_non_empty_spec l : ⟪Σ2_non_empty l⟫ = exists x, x ∈m ψ l.
+  Proof. reflexivity. Qed.
+
+  Fact Σ2_incl_spec x y : ⟪Σ2_incl x y⟫ = mb_incl mem (ψ x) (ψ y).
+  Proof. reflexivity. Qed.
+
+  Fact Σ2_equiv_spec x y : ⟪Σ2_equiv x y⟫ = mb_equiv mem (ψ x) (ψ y).
+  Proof. reflexivity. Qed. 
+
+  Fact Σ2_extensional_spec : ⟪Σ2_extensional⟫ = mb_member_ext mem.
+  Proof. reflexivity. Qed.
+
+  Fact Σ2_is_pair_spec p x y : ⟪Σ2_is_pair p x y⟫ = mb_is_pair mem (ψ p) (ψ x) (ψ y).
+  Proof. reflexivity. Qed.
+
+  Fact Σ2_is_otriple_spec p x y z : ⟪Σ2_is_otriple p x y z⟫ = mb_is_otriple mem (ψ p) (ψ x) (ψ y) (ψ z).
+  Proof. reflexivity. Qed.
+
+  Fact Σ2_is_otriple_in_spec r x y z : ⟪Σ2_is_otriple_in r x y z⟫ = mb_is_otriple_in mem (ψ r) (ψ x) (ψ y) (ψ z).
+  Proof. reflexivity. Qed.
+
+  Fact Σ2_has_otriples_spec l : ⟪Σ2_has_otriples l⟫ = mb_has_otriples mem (ψ l).
+  Proof. reflexivity. Qed.
+
+  Fact Σ2_list_in_spec l lv : ⟪Σ2_list_in l lv⟫ 
+                            <-> forall x, In x lv -> ψ x ∈m ψ l.
+  Proof.
+    induction lv as [ | x lv IH ]; simpl.
+    + split; tauto.
+    + split.
+      * intros (H1 & H2) ? [ <- | H ]; auto.
+        apply IH; auto.
+      * intros H; split.
+        - apply H; auto.
+        - apply IH; intros; apply H; auto.
+  Qed.
+
+End FOL_encoding. 
